Start an assembly model and remove JSON parsing

src/Assembly/Model.v
@@ -1,18 +1,16 @@
 Require Import Coq.ZArith.ZArith.
+Require Import Coq.NArith.NArith.
 Require Import Coq.Strings.String.
+Require Import Coq.Lists.List.
 Require Import Coq.Classes.Morphisms.
 Require Import Coq.Bool.Bool.
 Require Import Crypto.Util.Option.
 Require Import Crypto.Util.Bool.
 Require Import Crypto.Util.Bool.Reflect.
-(*
-Require Import Coq.Strings.String.
-Require Import Coq.Lists.List.
-Require Import Crypto.Util.Listable.
-Import ListNotations.
-Local Open Scope list_scope.
-Local Open Scope string_scope.
- *)
+Require Import Crypto.Util.ListUtil.
+Require Import Crypto.Util.Tactics.DestructHead.
+Require Crypto.Util.Tuple.
+
 Local Set Implicit Arguments.
 Local Set Boolean Equality Schemes.
 Local Set Decidable Equality Schemes.
@@ -25,47 +23,12 @@ Inductive REG :=
 | ah | al | ch | cl | dh | dl | bh | bl |  spl |  bpl |  sil |  dil | r8b | r9b | r10b | r11b | r12b | r13b | r14b | r15b
 .
 
-Declare Scope REG_scope.
-Delimit Scope REG_scope with REG.
-Bind Scope REG_scope with REG.
-
-Infix "=?" := REG_beq : REG_scope.
-
 Definition CONST := Z.
 Coercion CONST_of_Z (x : Z) : CONST := x.
 
-Definition CONST_beq : CONST -> CONST -> bool := Z.eqb.
-Definition CONST_dec_bl (x y : CONST) : CONST_beq x y = true -> x = y := proj1 (Z.eqb_eq x y).
-Definition CONST_dec_lb (x y : CONST) : x = y -> CONST_beq x y = true := proj2 (Z.eqb_eq x y).
-Definition CONST_eq_dec (x y : CONST) : {x = y} + {x <> y} := Z.eq_dec x y.
-
-Declare Scope CONST_scope.
-Delimit Scope CONST_scope with CONST.
-Bind Scope CONST_scope with CONST.
-
-Infix "=?" := CONST_beq : CONST_scope.
-
 Record MEM := { mem_is_byte : bool ; mem_reg : REG ; mem_extra_reg : option REG ; mem_offset : option Z }.
 
-Declare Scope MEM_scope.
-Delimit Scope MEM_scope with MEM.
-Bind Scope MEM_scope with MEM.
-
-Definition MEM_beq (x y : MEM) : bool
-  := ((bool_beq x.(mem_is_byte) y.(mem_is_byte))
-      && (x.(mem_reg) =? y.(mem_reg))%REG
-      && (option_beq REG_beq x.(mem_extra_reg) y.(mem_extra_reg))
-      && (option_beq Z.eqb x.(mem_offset) y.(mem_offset)))%bool.
-
-Infix "=?" := MEM_beq : MEM_scope.
-
 Inductive FLAG := CF | PF | AF | ZF | SF | OF.
-
-Declare Scope FLAG_scope.
-Delimit Scope FLAG_scope with FLAG.
-Bind Scope FLAG_scope with FLAG.
-
-Infix "=?" := FLAG_beq : FLAG_scope.
 
 Inductive OpCode :=
 | adc
@@ -95,33 +58,10 @@ Inductive OpCode :=
 | xor
 .
 
-Declare Scope OpCode_scope.
-Delimit Scope OpCode_scope with OpCode.
-Bind Scope OpCode_scope with OpCode.
-
-Infix "=?" := OpCode_beq : OpCode_scope.
-
 Inductive ARG := reg (r : REG) | mem (m : MEM) | const (c : CONST).
 Coercion reg : REG >-> ARG.
 Coercion mem : MEM >-> ARG.
 Coercion const : CONST >-> ARG.
-
-Declare Scope ARG_scope.
-Delimit Scope ARG_scope with ARG.
-Bind Scope ARG_scope with ARG.
-
-Definition ARG_beq (x y : ARG) : bool
-  := match x, y with
-     | reg x, reg y => REG_beq x y
-     | mem x, mem y => MEM_beq x y
-     | const x, const y => CONST_beq x y
-     | reg _, _
-     | mem _, _
-     | const _, _
-       => false
-     end.
-
-Infix "=?" := ARG_beq : ARG_scope.
 
 Record NormalInstruction := { op : OpCode ; args : list ARG }.
 
@@ -136,17 +76,10 @@ Coercion INSTR : NormalInstruction >-> RawLine.
 Record Line := { indent : string ; rawline :> RawLine ; pre_comment_whitespace : string ; comment : option string }.
 Definition Lines := list Line.
 
-(** denotational semantics *)
+Delimit Scope REG_scope with REG.
+Bind Scope REG_scope with REG.
 
-Record flag_state := { get_flag : FLAG -> option bool }.
-Definition set_flag_internal (st : flag_state) (f : FLAG) (v : option bool)
-  := {| get_flag f' := if f' =? f then v else st.(get_flag) f' |}%FLAG.
-Definition set_flag (st : flag_state) (f : FLAG) (v : bool)
-  := set_flag_internal st f (Some v).
-Definition havoc_flag (st : flag_state) (f : FLAG)
-  := set_flag_internal st f None.
-
-Record reg_state :=
+Infix "=?" := REG_beq : REG_scope.
 
 Global Instance REG_beq_spec : reflect_rel (@eq REG) REG_beq | 10
   := reflect_of_beq internal_REG_dec_bl internal_REG_dec_lb.
@@ -156,6 +89,16 @@ Proof. rewrite <- REG_beq_eq; destruct (x =? y)%REG; intuition congruence. Qed.
 Global Instance REG_beq_compat : Proper (eq ==> eq ==> eq) REG_beq | 10.
 Proof. repeat intro; subst; reflexivity. Qed.
 
+Definition CONST_beq : CONST -> CONST -> bool := Z.eqb.
+Definition CONST_dec_bl (x y : CONST) : CONST_beq x y = true -> x = y := proj1 (Z.eqb_eq x y).
+Definition CONST_dec_lb (x y : CONST) : x = y -> CONST_beq x y = true := proj2 (Z.eqb_eq x y).
+Definition CONST_eq_dec (x y : CONST) : {x = y} + {x <> y} := Z.eq_dec x y.
+
+Delimit Scope CONST_scope with CONST.
+Bind Scope CONST_scope with CONST.
+
+Infix "=?" := CONST_beq : CONST_scope.
+
 Global Instance CONST_beq_spec : reflect_rel (@eq CONST) CONST_beq | 10
   := reflect_of_beq CONST_dec_bl CONST_dec_lb.
 Definition CONST_beq_eq x y : (x =? y)%CONST = true <-> x = y := conj (@CONST_dec_bl _ _) (@CONST_dec_lb _ _).
@@ -164,11 +107,42 @@ Proof. rewrite <- CONST_beq_eq; destruct (x =? y)%CONST; intuition congruence. Q
 Global Instance CONST_beq_compat : Proper (eq ==> eq ==> eq) CONST_beq | 10.
 Proof. repeat intro; subst; reflexivity. Qed.
 
+Delimit Scope MEM_scope with MEM.
+Bind Scope MEM_scope with MEM.
+
+Definition MEM_beq (x y : MEM) : bool
+  := ((Bool.eqb x.(mem_is_byte) y.(mem_is_byte))
+      && (x.(mem_reg) =? y.(mem_reg))%REG
+      && (option_beq REG_beq x.(mem_extra_reg) y.(mem_extra_reg))
+      && (option_beq Z.eqb x.(mem_offset) y.(mem_offset)))%bool.
+Global Arguments MEM_beq !_ !_ / .
+
+Infix "=?" := MEM_beq : MEM_scope.
+
+Local Ltac t_dec :=
+  lazymatch goal with
+  | [ |- ?beq ?x ?y = true -> ?x = ?y ]
+    => is_var x; is_var y; destruct x, y; cbv [beq]
+  | [ |- ?x = ?y -> ?beq ?x ?y = true ]
+    => is_var x; is_var y; destruct x; cbv [beq]; intros; subst
+  end;
+  simpl;
+  rewrite ?Bool.andb_true_iff; intros; destruct_head'_and;
+  repeat apply conj; try reflexivity;
+  reflect_hyps; subst;
+  try solve [ reflexivity
+            | exfalso; assumption
+            | apply unreflect_bool; reflexivity ].
+
 Lemma MEM_dec_bl (x y : MEM) : MEM_beq x y = true -> x = y.
-Proof. destruct x, y; cbn.
-  := proj1 (Z.eqb_eq x y).
-Definition MEM_dec_lb (x y : MEM) : x = y -> MEM_beq x y = true := proj2 (Z.eqb_eq x y).
-Definition MEM_eq_dec (x y : MEM) : {x = y} + {x <> y} := Z.eq_dec x y.
+Proof. t_dec. Qed.
+Lemma MEM_dec_lb (x y : MEM) : x = y -> MEM_beq x y = true.
+Proof. t_dec. Qed.
+Definition MEM_eq_dec (x y : MEM) : {x = y} + {x <> y}
+  := (if (x =? y)%MEM as b return (x =? y)%MEM = b -> _
+      then fun pf => left (@MEM_dec_bl _ _ pf)
+      else fun pf => right (fun pf' => diff_false_true (eq_trans (eq_sym pf) (@MEM_dec_lb _ _ pf'))))
+       eq_refl.
 
 Global Instance MEM_beq_spec : reflect_rel (@eq MEM) MEM_beq | 10
   := reflect_of_beq MEM_dec_bl MEM_dec_lb.
@@ -178,78 +152,370 @@ Proof. rewrite <- MEM_beq_eq; destruct (x =? y)%MEM; intuition congruence. Qed.
 Global Instance MEM_beq_compat : Proper (eq ==> eq ==> eq) MEM_beq | 10.
 Proof. repeat intro; subst; reflexivity. Qed.
 
-Print internal_
+Delimit Scope FLAG_scope with FLAG.
+Bind Scope FLAG_scope with FLAG.
 
-Definition parse_quotes_around {A} (literal : ParserAction A) : ParserAction A
-  := """" ;;->{ fun _ v => v } literal ;;->{ fun v _ => v } """".
+Infix "=?" := FLAG_beq : FLAG_scope.
 
-Definition maybe_parse_quotes_around {A} (with_quotes : bool) : ParserAction A -> ParserAction A
-  := (if with_quotes then parse_quotes_around else fun x => x).
+Global Instance FLAG_beq_spec : reflect_rel (@eq FLAG) FLAG_beq | 10
+  := reflect_of_beq internal_FLAG_dec_bl internal_FLAG_dec_lb.
+Definition FLAG_beq_eq x y : (x =? y)%FLAG = true <-> x = y := conj (@internal_FLAG_dec_bl _ _) (@internal_FLAG_dec_lb _ _).
+Lemma FLAG_beq_neq x y : (x =? y)%FLAG = false <-> x <> y.
+Proof. rewrite <- FLAG_beq_eq; destruct (x =? y)%FLAG; intuition congruence. Qed.
+Global Instance FLAG_beq_compat : Proper (eq ==> eq ==> eq) FLAG_beq | 10.
+Proof. repeat intro; subst; reflexivity. Qed.
 
-Definition parse_REG_list : list (string * REG)
-  := Eval vm_compute in
-      List.map
-        (fun r => (show false r, r))
-        (list_all REG).
+Delimit Scope OpCode_scope with OpCode.
+Bind Scope OpCode_scope with OpCode.
 
-Definition parse_REG (with_quotes : bool) : ParserAction REG
-  := maybe_parse_quotes_around with_quotes (parse_strs parse_REG_list).
+Infix "=?" := OpCode_beq : OpCode_scope.
 
-Definition parse_FLAG_list : list (string * FLAG)
-  := Eval vm_compute in
-      List.map
-        (fun r => (show false r, r))
-        (list_all FLAG).
+Global Instance OpCode_beq_spec : reflect_rel (@eq OpCode) OpCode_beq | 10
+  := reflect_of_beq internal_OpCode_dec_bl internal_OpCode_dec_lb.
+Definition OpCode_beq_eq x y : (x =? y)%OpCode = true <-> x = y := conj (@internal_OpCode_dec_bl _ _) (@internal_OpCode_dec_lb _ _).
+Lemma OpCode_beq_neq x y : (x =? y)%OpCode = false <-> x <> y.
+Proof. rewrite <- OpCode_beq_eq; destruct (x =? y)%OpCode; intuition congruence. Qed.
+Global Instance OpCode_beq_compat : Proper (eq ==> eq ==> eq) OpCode_beq | 10.
+Proof. repeat intro; subst; reflexivity. Qed.
 
-Definition parse_FLAG (with_quotes : bool) : ParserAction FLAG
-  := maybe_parse_quotes_around with_quotes (parse_strs parse_FLAG_list).
+Delimit Scope ARG_scope with ARG.
+Bind Scope ARG_scope with ARG.
 
-Definition parse_MEM (with_quotes : bool) : ParserAction MEM
-  := maybe_parse_quotes_around
-       with_quotes
-       (parse_map
-          (fun '(has_byte, (r, (r', maybe_pm_z)))
-           => {| mem_is_byte := if has_byte:option _ then true else false
-                 ; mem_reg := r
-                 ; mem_extra_reg := r'
-                 ; mem_offset := match maybe_pm_z with
-                                 | inl (inl _ (* plus *), z) => Some z
-                                 | inl (inr _ (* minus *), z) => Some (-z)
-                                 | inr _ (* only whitespace *) => None
-                                 end%Z |})
-          (((strip_whitespace_after "byte ")?) ;;
-           (strip_whitespace_after "[" ;;R
-            parse_REG false ;;
-            ((strip_whitespace_around "+" ;;R parse_REG false)?) ;;
-            ((strip_whitespace_before ("+" ||->{id} "-") ;; parse_Z_arith_strict) ||->{id} parse_any_whitespace) ;;L
-            "]"))).
+Definition ARG_beq (x y : ARG) : bool
+  := match x, y with
+     | reg x, reg y => REG_beq x y
+     | mem x, mem y => MEM_beq x y
+     | const x, const y => CONST_beq x y
+     | reg _, _
+     | mem _, _
+     | const _, _
+       => false
+     end.
+Global Arguments ARG_beq !_ !_ / .
 
-Definition parse_CONST (const_keyword : bool) (with_quotes : bool) : ParserAction CONST
-  := maybe_parse_quotes_around
-       with_quotes
-       (if const_keyword
-        then "CONST " ;;R parse_Z_arith_strict ;;L parse_lookahead_not parse_one_whitespace
-        else parse_lookahead_not parse_one_whitespace ;;R parse_Z_arith_strict ;;L parse_lookahead_not parse_one_whitespace).
+Infix "=?" := ARG_beq : ARG_scope.
 
-Definition parse_ARG (const_keyword : bool) (with_quotes : bool) : ParserAction ARG
-  := parse_alt_list
-       [parse_map reg (parse_REG with_quotes)
-        ; parse_map mem (parse_MEM with_quotes)
-        ; parse_map const (parse_CONST const_keyword with_quotes)
-        ; parse_map flag (parse_FLAG with_quotes)].
+Lemma ARG_dec_bl (x y : ARG) : ARG_beq x y = true -> x = y.
+Proof. t_dec. Qed.
+Lemma ARG_dec_lb (x y : ARG) : x = y -> ARG_beq x y = true.
+Proof. t_dec. Qed.
+Definition ARG_eq_dec (x y : ARG) : {x = y} + {x <> y}
+  := (if (x =? y)%ARG as b return (x =? y)%ARG = b -> _
+      then fun pf => left (@ARG_dec_bl _ _ pf)
+      else fun pf => right (fun pf' => diff_false_true (eq_trans (eq_sym pf) (@ARG_dec_lb _ _ pf'))))
+       eq_refl.
 
-Definition parse_OpCode_list : list (string * OpCode)
-  := Eval vm_compute in
-      List.map
-        (fun r => (show false r, r))
-        (list_all OpCode).
+Global Instance ARG_beq_spec : reflect_rel (@eq ARG) ARG_beq | 10
+  := reflect_of_beq ARG_dec_bl ARG_dec_lb.
+Definition ARG_beq_eq x y : (x =? y)%ARG = true <-> x = y := conj (@ARG_dec_bl _ _) (@ARG_dec_lb _ _).
+Lemma ARG_beq_neq x y : (x =? y)%ARG = false <-> x <> y.
+Proof. rewrite <- ARG_beq_eq; destruct (x =? y)%ARG; intuition congruence. Qed.
+Global Instance ARG_beq_compat : Proper (eq ==> eq ==> eq) ARG_beq | 10.
+Proof. repeat intro; subst; reflexivity. Qed.
 
-Definition parse_OpCode (with_quotes : bool) : ParserAction OpCode
-  := maybe_parse_quotes_around with_quotes (parse_strs parse_OpCode_list).
+Delimit Scope NormalInstruction_scope with NormalInstruction.
+Bind Scope NormalInstruction_scope with NormalInstruction.
 
-Definition parse_name (with_quotes : bool) : ParserAction name
-  := maybe_parse_quotes_around
-       with_quotes
-       ((parse_map string_of_list_ascii ([a-zA-Z]+))
-          ;;->{ fun s n => {| name_prefix := s ; name_number := digits_to_N 10 n |} }
-          ((parse_digits_gen_step 10)* )).
+Definition NormalInstruction_beq (x y : NormalInstruction) : bool
+  := ((x.(op) =? y.(op))%OpCode
+      && list_beq _ ARG_beq x.(args) y.(args))%bool.
+Global Arguments NormalInstruction_beq !_ !_ / .
+
+Infix "=?" := NormalInstruction_beq : NormalInstruction_scope.
+
+Lemma NormalInstruction_dec_bl (x y : NormalInstruction) : NormalInstruction_beq x y = true -> x = y.
+Proof. t_dec. Qed.
+Lemma NormalInstruction_dec_lb (x y : NormalInstruction) : x = y -> NormalInstruction_beq x y = true.
+Proof. t_dec. Qed.
+Definition NormalInstruction_eq_dec (x y : NormalInstruction) : {x = y} + {x <> y}
+  := (if (x =? y)%NormalInstruction as b return (x =? y)%NormalInstruction = b -> _
+      then fun pf => left (@NormalInstruction_dec_bl _ _ pf)
+      else fun pf => right (fun pf' => diff_false_true (eq_trans (eq_sym pf) (@NormalInstruction_dec_lb _ _ pf'))))
+       eq_refl.
+
+Global Instance NormalInstruction_beq_spec : reflect_rel (@eq NormalInstruction) NormalInstruction_beq | 10
+  := reflect_of_beq NormalInstruction_dec_bl NormalInstruction_dec_lb.
+Definition NormalInstruction_beq_eq x y : (x =? y)%NormalInstruction = true <-> x = y := conj (@NormalInstruction_dec_bl _ _) (@NormalInstruction_dec_lb _ _).
+Lemma NormalInstruction_beq_neq x y : (x =? y)%NormalInstruction = false <-> x <> y.
+Proof. rewrite <- NormalInstruction_beq_eq; destruct (x =? y)%NormalInstruction; intuition congruence. Qed.
+Global Instance NormalInstruction_beq_compat : Proper (eq ==> eq ==> eq) NormalInstruction_beq | 10.
+Proof. repeat intro; subst; reflexivity. Qed.
+
+Delimit Scope RawLine_scope with RawLine.
+Bind Scope RawLine_scope with RawLine.
+
+Definition RawLine_beq (x y : RawLine) : bool
+  := match x, y with
+     | SECTION x, SECTION y => String.eqb x y
+     | GLOBAL x, GLOBAL y => String.eqb x y
+     | LABEL x, LABEL y => String.eqb x y
+     | EMPTY, EMPTY => true
+     | INSTR x, INSTR y => NormalInstruction_beq x y
+     | SECTION _, _
+     | GLOBAL _, _
+     | LABEL _, _
+     | EMPTY, _
+     | INSTR _, _
+       => false
+     end.
+Global Arguments RawLine_beq !_ !_ / .
+
+Infix "=?" := RawLine_beq : RawLine_scope.
+
+Lemma RawLine_dec_bl (x y : RawLine) : RawLine_beq x y = true -> x = y.
+Proof. t_dec. Qed.
+Lemma RawLine_dec_lb (x y : RawLine) : x = y -> RawLine_beq x y = true.
+Proof. t_dec. Qed.
+Definition RawLine_eq_dec (x y : RawLine) : {x = y} + {x <> y}
+  := (if (x =? y)%RawLine as b return (x =? y)%RawLine = b -> _
+      then fun pf => left (@RawLine_dec_bl _ _ pf)
+      else fun pf => right (fun pf' => diff_false_true (eq_trans (eq_sym pf) (@RawLine_dec_lb _ _ pf'))))
+       eq_refl.
+
+Global Instance RawLine_beq_spec : reflect_rel (@eq RawLine) RawLine_beq | 10
+  := reflect_of_beq RawLine_dec_bl RawLine_dec_lb.
+Definition RawLine_beq_eq x y : (x =? y)%RawLine = true <-> x = y := conj (@RawLine_dec_bl _ _) (@RawLine_dec_lb _ _).
+Lemma RawLine_beq_neq x y : (x =? y)%RawLine = false <-> x <> y.
+Proof. rewrite <- RawLine_beq_eq; destruct (x =? y)%RawLine; intuition congruence. Qed.
+Global Instance RawLine_beq_compat : Proper (eq ==> eq ==> eq) RawLine_beq | 10.
+Proof. repeat intro; subst; reflexivity. Qed.
+
+Delimit Scope Line_scope with Line.
+Bind Scope Line_scope with Line.
+
+Definition Line_beq (x y : Line) : bool
+  := ((x.(indent) =? y.(indent))%string
+      && (x.(rawline) =? y.(rawline))%RawLine
+      && (x.(pre_comment_whitespace) =? y.(pre_comment_whitespace))%string
+      && option_beq String.eqb x.(comment) y.(comment))%bool.
+Global Arguments Line_beq !_ !_ / .
+
+Infix "=?" := Line_beq : Line_scope.
+
+Lemma Line_dec_bl (x y : Line) : Line_beq x y = true -> x = y.
+Proof. t_dec. Qed.
+Lemma Line_dec_lb (x y : Line) : x = y -> Line_beq x y = true.
+Proof. t_dec. Qed.
+Definition Line_eq_dec (x y : Line) : {x = y} + {x <> y}
+  := (if (x =? y)%Line as b return (x =? y)%Line = b -> _
+      then fun pf => left (@Line_dec_bl _ _ pf)
+      else fun pf => right (fun pf' => diff_false_true (eq_trans (eq_sym pf) (@Line_dec_lb _ _ pf'))))
+       eq_refl.
+
+Global Instance Line_beq_spec : reflect_rel (@eq Line) Line_beq | 10
+  := reflect_of_beq Line_dec_bl Line_dec_lb.
+Definition Line_beq_eq x y : (x =? y)%Line = true <-> x = y := conj (@Line_dec_bl _ _) (@Line_dec_lb _ _).
+Lemma Line_beq_neq x y : (x =? y)%Line = false <-> x <> y.
+Proof. rewrite <- Line_beq_eq; destruct (x =? y)%Line; intuition congruence. Qed.
+Global Instance Line_beq_compat : Proper (eq ==> eq ==> eq) Line_beq | 10.
+Proof. repeat intro; subst; reflexivity. Qed.
+
+Delimit Scope Lines_scope with Lines.
+Bind Scope Lines_scope with Lines.
+
+Definition Lines_beq (x y : Lines) : bool
+  := list_beq _ Line_beq x y.
+Global Arguments Lines_beq !_ !_ / .
+
+Infix "=?" := Lines_beq : Lines_scope.
+
+Lemma Lines_dec_bl (x y : Lines) : Lines_beq x y = true -> x = y.
+Proof. t_dec. Qed.
+Lemma Lines_dec_lb (x y : Lines) : x = y -> Lines_beq x y = true.
+Proof. t_dec. Qed.
+Definition Lines_eq_dec (x y : Lines) : {x = y} + {x <> y}
+  := (if (x =? y)%Lines as b return (x =? y)%Lines = b -> _
+      then fun pf => left (@Lines_dec_bl _ _ pf)
+      else fun pf => right (fun pf' => diff_false_true (eq_trans (eq_sym pf) (@Lines_dec_lb _ _ pf'))))
+       eq_refl.
+
+Global Instance Lines_beq_spec : reflect_rel (@eq Lines) Lines_beq | 10
+  := reflect_of_beq Lines_dec_bl Lines_dec_lb.
+Definition Lines_beq_eq x y : (x =? y)%Lines = true <-> x = y := conj (@Lines_dec_bl _ _) (@Lines_dec_lb _ _).
+Lemma Lines_beq_neq x y : (x =? y)%Lines = false <-> x <> y.
+Proof. rewrite <- Lines_beq_eq; destruct (x =? y)%Lines; intuition congruence. Qed.
+Global Instance Lines_beq_compat : Proper (eq ==> eq ==> eq) Lines_beq | 10.
+Proof. repeat intro; subst; reflexivity. Qed.
+
+(** denotational semantics *)
+
+Definition flag_state := Tuple.tuple (option bool) 6.
+Definition get_flag (st : flag_state) (f : FLAG) : option bool
+  := let '(cfv, pfv, afv, zfv, sfv, ofv) := st in
+     match f with
+     | CF => cfv
+     | PF => pfv
+     | AF => afv
+     | ZF => zfv
+     | SF => sfv
+     | OF => ofv
+     end.
+Definition set_flag_internal (st : flag_state) (f : FLAG) (v : option bool) : flag_state
+  := let '(cfv, pfv, afv, zfv, sfv, ofv) := st in
+     (match f with CF => v | _ => cfv end,
+      match f with PF => v | _ => pfv end,
+      match f with AF => v | _ => afv end,
+      match f with ZF => v | _ => zfv end,
+      match f with SF => v | _ => sfv end,
+      match f with OF => v | _ => ofv end).
+Definition set_flag (st : flag_state) (f : FLAG) (v : bool) : flag_state
+  := set_flag_internal st f (Some v).
+Definition havoc_flag (st : flag_state) (f : FLAG) : flag_state
+  := set_flag_internal st f None.
+Definition havoc_flags (st : flag_state) : flag_state
+  := (None, None, None, None, None, None).
+
+Definition reg_state := list N.
+Definition index_and_shift_and_bitcount_of_reg (r : REG) : nat * N * N
+  := (match r with
+      |     rax
+      |     eax
+      |      ax
+      |(ah | al)
+       => 0
+      |     rcx
+      |     ecx
+      |      cx
+      |(ch | cl)
+       => 1
+      |     rdx
+      |     edx
+      |      dx
+      |(dh | dl)
+       => 2
+      |     rbx
+      |     ebx
+      |      bx
+      |(bh | bl)
+       => 3
+      | rsp
+      | esp
+      |  sp
+      |( spl)
+       => 4
+      | rbp
+      | ebp
+      |  bp
+      |( bpl)
+       => 5
+      | rsi
+      | esi
+      |  si
+      |( sil)
+       => 6
+      | rdi
+      | edi
+      |  di
+      |( dil)
+       => 7
+      | r8
+      | r8d
+      | r8w
+      | r8b
+        => 8
+      | r9
+      | r9d
+      | r9w
+      | r9b
+        => 9
+      | r10
+      | r10d
+      | r10w
+      | r10b
+        => 10
+      | r11
+      | r11d
+      | r11w
+      | r11b
+        => 11
+      | r12
+      | r12d
+      | r12w
+      | r12b
+        => 12
+      | r13
+      | r13d
+      | r13w
+      | r13b
+        => 13
+      | r14
+      | r14d
+      | r14w
+      | r14b
+        => 14
+      | r15
+      | r15d
+      | r15w
+      | r15b
+        => 15
+      end,
+      match r with
+      |(    rax |     rcx |     rdx |     rbx | rsp  | rbp  | rsi  | rdi  | r8  | r9  | r10  | r11  | r12  | r13  | r14  | r15 )
+      |(    eax |     ecx |     edx |     ebx | esp  | ebp  | esi  | edi  | r8d | r9d | r10d | r11d | r12d | r13d | r14d | r15d)
+      |(     ax |      cx |      dx |      bx |  sp  |  bp  |  si  |  di  | r8w | r9w | r10w | r11w | r12w | r13w | r14w | r15w)
+      |(     al |      cl |      dl |      bl |  spl |  bpl |  sil |  dil | r8b | r9b | r10b | r11b | r12b | r13b | r14b | r15b)
+       => 0
+      |(ah      | ch      | dh      | bh      )
+       => 8
+      end%N,
+      match r with
+      |(    rax |     rcx |     rdx |     rbx | rsp  | rbp  | rsi  | rdi  | r8  | r9  | r10  | r11  | r12  | r13  | r14  | r15 )
+       => 64
+      |(    eax |     ecx |     edx |     ebx | esp  | ebp  | esi  | edi  | r8d | r9d | r10d | r11d | r12d | r13d | r14d | r15d)
+       => 32
+      |(     ax |      cx |      dx |      bx |  sp  |  bp  |  si  |  di  | r8w | r9w | r10w | r11w | r12w | r13w | r14w | r15w)
+       => 16
+      |(ah | al | ch | cl | dh | dl | bh | bl |  spl |  bpl |  sil |  dil | r8b | r9b | r10b | r11b | r12b | r13b | r14b | r15b)
+       => 8
+      end%N).
+Definition bitmask_of_reg (r : REG) : N
+  := let '(idx, shift, bitcount) := index_and_shift_and_bitcount_of_reg r in
+     N.shiftl (N.ones bitcount) shift.
+Definition get_reg (st : reg_state) (r : REG) : N
+  := let '(idx, shift, bitcount) := index_and_shift_and_bitcount_of_reg r in
+     let rv := nth_default 0%N st idx in
+     N.land (N.shiftr rv shift) (N.ones bitcount).
+Definition set_reg (st : reg_state) (r : REG) (v : N) : reg_state
+  := let '(idx, shift, bitcount) := index_and_shift_and_bitcount_of_reg r in
+     let bitmask := bitmask_of_reg r in
+     ListUtil.update_nth
+       idx
+       (fun curv => N.lor (N.land bitmask (N.shiftl v shift))
+                          (N.ldiff curv bitmask))
+       st.
+
+Record machine_state := { machine_reg_state :> reg_state ; machine_flag_state :> flag_state }.
+Definition update_reg_with (st : machine_state) (f : reg_state -> reg_state) : machine_state
+  := {| machine_reg_state := f st.(machine_reg_state) ; machine_flag_state := st.(machine_flag_state) |}.
+Definition update_flag_with (st : machine_state) (f : flag_state -> flag_state) : machine_state
+  := {| machine_reg_state := st.(machine_reg_state) ; machine_flag_state := f st.(machine_flag_state) |}.
+(*
+Definition DenoteNormalInstruction (st : machine_state) (instr : NormalInstruction) : option machine_state.
+  refine match instr.(op), instr.(args) with
+         | adc, _ => _
+         | adcx, _ => _
+         | add, _ => _
+         | adox, _ => _
+         | and, _ => _
+         | clc, _ => _
+         | cmovnz, _ => _
+         | dec, _ => _
+         | imul, _ => _
+         | inc, _ => _
+         | lea, _ => _
+         | mov, _ => _
+         | movzx, _ => _
+         | mulx, _ => _
+         | ret, _ => _
+         | sar, _ => _
+         | sbb, _ => _
+         | setc, _ => _
+         | seto, _ => _
+         | shr, _ => _
+         | shrd, _ => _
+         | sub, _ => _
+         | test, _ => _
+         | xchg, _ => _
+         | xor, _ => _
+         end.
+*)
