src/Assembly/Parse.v
@@ -1,33 +1,205 @@
 Require Import Coq.ZArith.ZArith.
+Require Import Coq.derive.Derive.
 Require Import Coq.Strings.String.
 Require Import Coq.Lists.List.
-Require Import Crypto.Util.Strings.Parse.Common.
-Require Import Crypto.Util.Strings.String.
+Require Import Crypto.Assembly.Model.
 Require Import Crypto.Util.OptionList.
-Require Import Crypto.Assembly.Parse.Common.
-Require Import Crypto.Util.ErrorT.
+Require Import Crypto.Util.Strings.Parse.Common.
+Require Import Crypto.Util.Strings.ParseArithmetic.
+Require Import Crypto.Util.Strings.String.
 Require Import Crypto.Util.Strings.Show.
+Require Import Crypto.Util.Listable.
+Require Import Crypto.Util.ErrorT.
 Require Import Crypto.Util.ListUtil.
 Import ListNotations.
 Local Open Scope list_scope.
 Local Open Scope string_scope.
 Local Open Scope parse_scope.
 
-Local Set Boolean Equality Schemes.
-Local Set Decidable Equality Schemes.
+Derive REG_Listable SuchThat (@FinitelyListable REG REG_Listable) As REG_FinitelyListable.
+Proof. prove_ListableDerive. Qed.
+Global Existing Instances REG_Listable REG_FinitelyListable.
 
-Record NormalInstruction := { op : OpCode ; args : list ARG }.
+(* M-x query-replace-regex RET ([^ ]+) => _ RET \1 => "\1" *)
+Global Instance show_REG : Show REG
+  := fun with_parens reg
+     => match reg with
+        | rax => "rax"
+        | rcx => "rcx"
+        | rdx => "rdx"
+        | rbx => "rbx"
+        | rsp => "rsp"
+        | rbp => "rbp"
+        | rsi => "rsi"
+        | rdi => "rdi"
+        | r8 => "r8"
+        | r9 => "r9"
+        | r10 => "r10"
+        | r11 => "r11"
+        | r12 => "r12"
+        | r13 => "r13"
+        | r14 => "r14"
+        | r15 => "r15"
+        | eax => "eax"
+        | ecx => "ecx"
+        | edx => "edx"
+        | ebx => "ebx"
+        | esp => "esp"
+        | ebp => "ebp"
+        | esi => "esi"
+        | edi => "edi"
+        | r8d => "r8d"
+        | r9d => "r9d"
+        | r10d => "r10d"
+        | r11d => "r11d"
+        | r12d => "r12d"
+        | r13d => "r13d"
+        | r14d => "r14d"
+        | r15d => "r15d"
+        | ax => "ax"
+        | cx => "cx"
+        | dx => "dx"
+        | bx => "bx"
+        | sp => "sp"
+        | bp => "bp"
+        | si => "si"
+        | di => "di"
+        | r8w => "r8w"
+        | r9w => "r9w"
+        | r10w => "r10w"
+        | r11w => "r11w"
+        | r12w => "r12w"
+        | r13w => "r13w"
+        | r14w => "r14w"
+        | r15w => "r15w"
+        | ah => "ah"
+        | al => "al"
+        | ch => "ch"
+        | cl => "cl"
+        | dh => "dh"
+        | dl => "dl"
+        | bh => "bh"
+        | bl => "bl"
+        | spl => "spl"
+        | bpl => "bpl"
+        | sil => "sil"
+        | dil => "dil"
+        | r8b => "r8b"
+        | r9b => "r9b"
+        | r10b => "r10b"
+        | r11b => "r11b"
+        | r12b => "r12b"
+        | r13b => "r13b"
+        | r14b => "r14b"
+        | r15b => "r15b"
+        end.
 
-Inductive RawLine :=
-| SECTION (name : string)
-| GLOBAL (name : string)
-| LABEL (name : string)
-| EMPTY
-| INSTR (instr : NormalInstruction)
-.
-Coercion INSTR : NormalInstruction >-> RawLine.
-Record Line := { indent : string ; rawline :> RawLine ; pre_comment_whitespace : string ; comment : option string }.
-Definition Lines := list Line.
+Derive FLAG_Listable SuchThat (@FinitelyListable FLAG FLAG_Listable) As FLAG_FinitelyListable.
+Proof. prove_ListableDerive. Qed.
+Global Existing Instances FLAG_Listable FLAG_FinitelyListable.
+
+(* M-x query-replace-regex RET ([^ ]+) => _ RET \1 => "\1" *)
+Global Instance show_FLAG : Show FLAG
+  := fun with_parens flag
+     => match flag with
+        | CF => "CF"
+        | PF => "PF"
+        | AF => "AF"
+        | ZF => "ZF"
+        | SF => "SF"
+        | OF => "OF"
+        end.
+
+Derive OpCode_Listable SuchThat (@FinitelyListable OpCode OpCode_Listable) As OpCode_FinitelyListable.
+Proof. prove_ListableDerive. Qed.
+Global Existing Instances OpCode_Listable OpCode_FinitelyListable.
+
+(* M-x query-replace-regex RET ([^ ]+) => _ RET \1 => "\1" *)
+Global Instance show_OpCode : Show OpCode
+  := fun with_parens opc
+     => match opc with
+        | adc => "adc"
+        | adcx => "adcx"
+        | add => "add"
+        | adox => "adox"
+        | and => "and"
+        | clc => "clc"
+        | cmovnz => "cmovnz"
+        | dec => "dec"
+        | imul => "imul"
+        | inc => "inc"
+        | lea => "lea"
+        | mov => "mov"
+        | movzx => "movzx"
+        | mulx => "mulx"
+        | ret => "ret"
+        | sar => "sar"
+        | sub => "sub"
+        | sbb => "sbb"
+        | setc => "setc"
+        | seto => "seto"
+        | shrd => "shrd"
+        | shr => "shr"
+        | test => "test"
+        | xchg => "xchg"
+        | xor => "xor"
+        end.
+
+Definition parse_REG_list : list (string * REG)
+  := Eval vm_compute in
+      List.map
+        (fun r => (show false r, r))
+        (list_all REG).
+
+Definition parse_REG : ParserAction REG
+  := parse_strs parse_REG_list.
+
+Definition parse_FLAG_list : list (string * FLAG)
+  := Eval vm_compute in
+      List.map
+        (fun r => (show false r, r))
+        (list_all FLAG).
+
+Definition parse_FLAG : ParserAction FLAG
+  := parse_strs parse_FLAG_list.
+
+Definition parse_MEM : ParserAction MEM
+  := parse_map
+        (fun '(has_byte, (r, (r', maybe_pm_z)))
+         => {| mem_is_byte := if has_byte:option _ then true else false
+               ; mem_reg := r
+               ; mem_extra_reg := r'
+               ; mem_offset := match maybe_pm_z with
+                               | inl (inl _ (* plus *), z) => Some z
+                               | inl (inr _ (* minus *), z) => Some (-z)
+                               | inr _ (* only whitespace *) => None
+                               end%Z |})
+        (((strip_whitespace_after "byte ")?) ;;
+         (strip_whitespace_after "[" ;;R
+          parse_REG ;;
+          ((strip_whitespace_around "+" ;;R parse_REG)?) ;;
+          ((strip_whitespace_before ("+" ||->{id} "-") ;; parse_Z_arith_strict) ||->{id} parse_any_whitespace) ;;L
+          "]")).
+
+Definition parse_CONST (const_keyword : bool) : ParserAction CONST
+  := if const_keyword
+     then "CONST " ;;R parse_Z_arith_strict ;;L parse_lookahead_not parse_one_whitespace
+     else parse_lookahead_not parse_one_whitespace ;;R parse_Z_arith_strict ;;L parse_lookahead_not parse_one_whitespace.
+
+Definition parse_ARG (const_keyword : bool) : ParserAction ARG
+  := parse_alt_list
+       [parse_map reg parse_REG
+        ; parse_map mem parse_MEM
+        ; parse_map const (parse_CONST const_keyword)].
+
+Definition parse_OpCode_list : list (string * OpCode)
+  := Eval vm_compute in
+      List.map
+        (fun r => (show false r, r))
+        (list_all OpCode).
+
+Definition parse_OpCode : ParserAction OpCode
+  := parse_strs parse_OpCode_list.
 
 (** assumes no leading nor trailing whitespace and no comment *)
 Definition parse_RawLine : ParserAction RawLine
@@ -44,8 +216,8 @@ Definition parse_RawLine : ParserAction RawLine
                   then [(LABEL (substring 0 (pred (String.length s)) s), "")]
                   else if (s =? "")
                        then [(EMPTY, "")]
-                       else let parsed_mnemonic := (parse_OpCode false ;;L ε) mnemonic in
-                            let parsed_args := (parse_list_gen "" "," "" (parse_ARG false false) ;;L ε) args in
+                       else let parsed_mnemonic := (parse_OpCode ;;L ε) mnemonic in
+                            let parsed_args := (parse_list_gen "" "," "" (parse_ARG false) ;;L ε) args in
                             List.flat_map
                               (fun '(opc, _)
                                => List.map
@@ -113,7 +285,6 @@ Global Instance show_ARG : Show ARG
         | reg r => show with_parens r
         | mem m => show with_parens m
         | const c => show with_parens c
-        | flag f => show with_parens f
         end.
 
 Global Instance show_NormalInstruction : Show NormalInstruction
@@ -142,10 +313,6 @@ Global Instance show_Line : Show Line
 
 Global Instance show_lines_Lines : ShowLines Lines
   := fun with_parens ls => List.map (show false) ls.
-
-Definition Lines_beq : Lines -> Lines -> bool := list_beq _ Line_beq.
-Lemma Lines_beq_eq x y : Lines_beq x y = true <-> x = y.
-Proof. cbv [Lines_beq]; split; first [ apply internal_list_dec_lb | apply internal_list_dec_bl ]. Abort.
 
 Definition parse_correct_on (v : list string)
   := forall res, parse v = Success res -> parse v = parse (show_lines false res).
